More progress on AVL implementation

examples/steel/FStar.Trees.fst
@@ -73,13 +73,6 @@ let rec height (#a: Type) (x: tree a) : nat =
     if height left > height right then (height left) + 1
     else (height right) + 1
 
-let is_balanced (#a: Type) (x: tree a) : prop =
-  match x with
-  | Leaf -> True
-  | Node data left right ->
-    (height left - height right) <= 1 /\
-    (height right - height left) <= 1
-
 (**** Append *)
 
 let rec append_left (#a: Type) (x: tree a) (v: a) : tree a =
@@ -152,34 +145,7 @@ let rec insert_bst_preserves_bst
 
 (**** AVL Trees *)
 
-(* An AVL is a key-value tree where the value is the node's height. *)
-let avl (a: Type) {| d: ordered a |} = x: kv_tree a int {is_bst x}
-
-let get_payload (#a: Type) (x: kv_tree a int) : int =
-  match x with
-  | Leaf -> 0
-  | Node data left right -> data.payload
-  
-let balance_factor (#a: Type) (x: kv_tree a int) : int =
-  match x with
-  | Leaf -> 0
-  | Node data left right -> get_payload(right) - get_payload(left)
-
-// Takes in two nodes, returns max(height l, height r) + 1
-let compute_parent_height (#a: Type) (l r: kv_tree a int) : int =
-  if get_payload(l) > get_payload(r) then (
-    get_payload(l) + 1
-  ) else (
-    get_payload(r) + 1
-  )
-  
-// let rotate_left (#a: Type) (r: kv_tree a int) : option (avl a) =
-//   match r with
-//   | Node x t1 (Node z t2 t3) -> 
-//     let x' = Node ({x.key; compute_parent_height(t1, t2)}) t1 t2 in
-//     let z' = ({z.key; compute_parent_height(x', t3)}) in
-//     Some (Node z' x' t3)
-//   | _ -> None
+let avl (a b: Type) {| d: ordered a |} = x: kv_tree a b {is_bst x}
 
 let rotate_left (#a: Type) (r: tree a) : option (tree a) =
   match r with
@@ -201,12 +167,12 @@ let rotate_left_right (#a: Type) (r: tree a) : option (tree a) =
   | Node x (Node z t1 (Node y t2 t3)) t4 -> Some (Node y (Node z t1 t2) (Node x t3 t4))
   | _ -> None
 
-let rebalance_avl (#a: Type) {| d: ordered a |} (x: kv_tree a int) : kv_tree a int =
+let rebalance_avl (#a #b: Type) {| d: ordered a |} (x: kv_tree a b) : kv_tree a b =
     match x with
     | Leaf -> x
     | Node data left right ->
  
-      if balance_factor(x) > 1 then (
+      if (height right - height left) > 1 then (
       match left with
       | Node ldata lleft lright ->
         if d.compare data.key ldata.key > 0 then (
@@ -223,7 +189,7 @@ let rebalance_avl (#a: Type) {| d: ordered a |} (x: kv_tree a int) : kv_tree a i
       | _ -> x
 
     ) else (
-      if balance_factor(x) < -1 then (
+      if (height right - height left) < -1 then (
         match right with
         | Node rdata rleft rright ->
           if d.compare data.key rdata.key > 0 then (
@@ -243,17 +209,29 @@ let rebalance_avl (#a: Type) {| d: ordered a |} (x: kv_tree a int) : kv_tree a i
       )
     )
     
-let rec insert_avl (#a: Type) {| d: ordered a |} (x: avl a) (key: a) : kv_tree a int =
+let rec insert_avl (#a #b: Type) {| d: ordered a |} (x: avl a b) (key: a) (payload: b): kv_tree a b =
   match x with
-  | Leaf -> Node ({key; payload=0}) Leaf Leaf
+  | Leaf -> Node ({key; payload}) Leaf Leaf
   | Node data left right ->
     let delta = d.compare data.key key in
     if delta >= 0 then (
-      let new_left = insert_avl left key in
+      let new_left = insert_avl left key payload in
       let tmp = Node data new_left right in
       rebalance_avl(tmp)
     ) else (
-      let new_right = insert_avl right key in
+      let new_right = insert_avl right key payload in
       let tmp = Node data left new_right in
       rebalance_avl(tmp)
     )
+
+let rec is_balanced (#a: Type) (x: tree a) : prop =
+  match x with
+  | Leaf -> True
+  | Node data left right ->
+    (height left - height right) <= 1 /\
+    (height right - height left) <= 1 /\
+    is_balanced(right) /\
+    is_balanced(left)
+
+let is_avl (#a #b: Type) {| d: ordered a |} (x: kv_tree a b) : prop =
+  is_bst(x) /\ is_balanced(x)
