examples/steel/Selectors.Tree.fsti
@@ -65,3 +65,17 @@ val rotate_left_right (#a: Type) (ptr: t a)
     (ensures (fun h0 ptr' h1 ->
         Spec.rotate_left_right (v_linked_tree ptr h0) == Some (v_linked_tree ptr' h1)
     ))
+
+val rebalance_avl (#a: Type) (ptr: t a)
+    : SteelSel (t a) (linked_tree ptr) (fun ptr' -> linked_tree ptr')
+    (requires fun h0 -> Spec.is_bst(v_linked_tree ptr h0)
+    (ensures fun h0 ptr' h1 ->
+        Spec.rebalance_avl (v_linked_tree ptr h0) == v_linked_tree ptr' h1 /\
+        is_avl (v_linked_tree ptr' h1))
+
+val insert_avl (#a: Type) (ptr: t a)
+    : SteelSel (t a) (linked_tree ptr) (fun ptr' -> linked_tree ptr')
+    (requires fun h0 -> Spec.is_avl(v_linked_tree ptr h0)
+    (ensures fun h0 ptr' h1 ->
+        Spec.insert_avl (v_linked_tree ptr h0) == v_linked_tree ptr' h1 /\
+        is_avl (v_linked_tree ptr' h1))
